@prefix owl: <http://www.w3.org/2002/07/owl#> .
@prefix rdfs: <http://www.w3.org/2000/01/rdf-schema#> .
@prefix xsd: <http://www.w3.org/2001/XMLSchema#> .

<http://www.semanticweb.org/joliendeclerck/ontologies/2016/3/OIS-food-ontology> 
	a owl:Ontology ;
	owl:imports <file:///home/arno/workspace/Open%20information%20systems/db2triple/output.ttl> .
<http://www.semanticweb.org/joliendeclerck/ontologies/2016/3/OIS-food-ontology#hasIngredient>
  a owl:ObjectProperty ;
  rdfs:domain <http://www.semanticweb.org/joliendeclerck/ontologies/2016/3/OIS-food-ontology#IngredientQuantity> ;
  rdfs:range <http://www.semanticweb.org/joliendeclerck/ontologies/2016/3/OIS-food-ontology#Ingredient> ;
  rdfs:comment "an ingredient quantity references to the quantity of some ingredient" ;
  rdfs:label "has ingredient" .

<http://www.semanticweb.org/joliendeclerck/ontologies/2016/3/OIS-food-ontology#hasNutrititiveValueQuantity>
  a owl:ObjectProperty ;
  rdfs:domain <http://www.semanticweb.org/joliendeclerck/ontologies/2016/3/OIS-food-ontology#Ingredient> ;
  rdfs:range <http://www.semanticweb.org/joliendeclerck/ontologies/2016/3/OIS-food-ontology#NutritiveValueQuantity> ;
  rdfs:comment "an ingredient has multiple nutritive value quantities" ;
  rdfs:label "has nutritive value quantity" .

<http://www.semanticweb.org/joliendeclerck/ontologies/2016/3/OIS-food-ontology#hasNutritiveValue>
  a owl:ObjectProperty ;
  rdfs:domain <http://www.semanticweb.org/joliendeclerck/ontologies/2016/3/OIS-food-ontology#NutritiveValueQuantity> ;
  rdfs:range <http://www.semanticweb.org/joliendeclerck/ontologies/2016/3/OIS-food-ontology#NutritiveValue> ;
  rdfs:comment "the nutritive value for a certain nutritive value quantity" ;
  rdfs:label "has nutritive value" .

<http://www.semanticweb.org/joliendeclerck/ontologies/2016/3/OIS-food-ontology#hasStep>
  a owl:ObjectProperty ;
  rdfs:domain <http://www.semanticweb.org/joliendeclerck/ontologies/2016/3/OIS-food-ontology#Recipe> ;
  rdfs:range <http://www.semanticweb.org/joliendeclerck/ontologies/2016/3/OIS-food-ontology#RecipeStep> ;
  rdfs:comment "a recipe can consists of some steps" ;
  rdfs:label "has step" .

<http://www.semanticweb.org/joliendeclerck/ontologies/2016/3/OIS-food-ontology#requiresQuantityOfIngredient>
  a owl:ObjectProperty ;
  rdfs:domain <http://www.semanticweb.org/joliendeclerck/ontologies/2016/3/OIS-food-ontology#Recipe> ;
  rdfs:range <http://www.semanticweb.org/joliendeclerck/ontologies/2016/3/OIS-food-ontology#IngredientQuantity> ;
  rdfs:comment "a recipe requires a quantity of an ingredient" ;
  rdfs:label "requires quantity of ingredient" .

<http://www.semanticweb.org/joliendeclerck/ontologies/2016/3/OIS-food-ontology#resultsIn>
  a owl:ObjectProperty ;
  rdfs:domain <http://www.semanticweb.org/joliendeclerck/ontologies/2016/3/OIS-food-ontology#Recipe> ;
  rdfs:range <http://www.semanticweb.org/joliendeclerck/ontologies/2016/3/OIS-food-ontology#Food> ;
  rdfs:comment "food can be the result of a recipe" ;
  rdfs:label "results in" .

<http://www.semanticweb.org/joliendeclerck/ontologies/2016/3/OIS-food-ontology#hasBrand>
  a owl:DatatypeProperty ;
  rdfs:domain <http://www.semanticweb.org/joliendeclerck/ontologies/2016/3/OIS-food-ontology#Ingredient> ;
  rdfs:range xsd:string ;
  rdfs:comment "an ingredient can have a brand" ;
  rdfs:label "has brand" .

<http://www.semanticweb.org/joliendeclerck/ontologies/2016/3/OIS-food-ontology#hasFoodName>
  a owl:DatatypeProperty ;
  rdfs:domain <http://www.semanticweb.org/joliendeclerck/ontologies/2016/3/OIS-food-ontology#Food> ;
  rdfs:range xsd:string ;
  rdfs:comment "a food has a name" ;
  rdfs:label "has food name" .

<http://www.semanticweb.org/joliendeclerck/ontologies/2016/3/OIS-food-ontology#hasIngredientName>
  a owl:DatatypeProperty ;
  rdfs:domain <http://www.semanticweb.org/joliendeclerck/ontologies/2016/3/OIS-food-ontology#Ingredient> ;
  rdfs:range xsd:string ;
  rdfs:comment "an ingredient has a name" ;
  rdfs:label "has ingredient name" .

<http://www.semanticweb.org/joliendeclerck/ontologies/2016/3/OIS-food-ontology#hasIngredientQuantity>
  a owl:DatatypeProperty ;
  rdfs:domain <http://www.semanticweb.org/joliendeclerck/ontologies/2016/3/OIS-food-ontology#IngredientQuantity> ;
  rdfs:range xsd:float ;
  rdfs:comment "this number specifies the required quantity of some ingredient in the recipe" ;
  rdfs:label "has ingredient quantity" .

<http://www.semanticweb.org/joliendeclerck/ontologies/2016/3/OIS-food-ontology#hasNutrientQuantityUnit>
  a owl:DatatypeProperty ;
  rdfs:domain <http://www.semanticweb.org/joliendeclerck/ontologies/2016/3/OIS-food-ontology#NutritiveValueQuantity> ;
  rdfs:range xsd:string ;
  rdfs:comment "the unit in which a certain nutritive value is expressed" ;
  rdfs:label "has nutritive quantity unit" .

<http://www.semanticweb.org/joliendeclerck/ontologies/2016/3/OIS-food-ontology#hasNutritiveQuantity>
  a owl:DatatypeProperty ;
  rdfs:domain <http://www.semanticweb.org/joliendeclerck/ontologies/2016/3/OIS-food-ontology#NutritiveValueQuantity> ;
  rdfs:range xsd:float ;
  rdfs:comment "the quantity of a nutritive value that is present in 100 grams of a certain ingredient" ;
  rdfs:label "has nutritive quantity" .

<http://www.semanticweb.org/joliendeclerck/ontologies/2016/3/OIS-food-ontology#hasNutritiveValueName>
  a owl:DatatypeProperty ;
  rdfs:domain <http://www.semanticweb.org/joliendeclerck/ontologies/2016/3/OIS-food-ontology#NutritiveValue> ;
  rdfs:range xsd:string ;
  rdfs:comment "a name for a nutritive value." ;
  rdfs:label "has nutritive value name" .

<http://www.semanticweb.org/joliendeclerck/ontologies/2016/3/OIS-food-ontology#hasOrderingNumber>
  a owl:DatatypeProperty ;
  rdfs:domain <http://www.semanticweb.org/joliendeclerck/ontologies/2016/3/OIS-food-ontology#RecipeStep> ;
  rdfs:range xsd:integer ;
  rdfs:comment """the number indicates the order in which this step needs to be completed
in order to complete the recipe""" ;
  rdfs:label "has ordering number" .

<http://www.semanticweb.org/joliendeclerck/ontologies/2016/3/OIS-food-ontology#hasQuantityUnit>
  a owl:DatatypeProperty ;
  rdfs:domain <http://www.semanticweb.org/joliendeclerck/ontologies/2016/3/OIS-food-ontology#IngredientQuantity> ;
  rdfs:range xsd:string ;
  rdfs:comment "the unit specifying the quantity for an ingredient, for example gram" ;
  rdfs:label "has quantity unit" .

<http://www.semanticweb.org/joliendeclerck/ontologies/2016/3/OIS-food-ontology#hasStepDescription>
  a owl:DatatypeProperty ;
  rdfs:domain <http://www.semanticweb.org/joliendeclerck/ontologies/2016/3/OIS-food-ontology#RecipeStep> ;
  rdfs:range xsd:string ;
  rdfs:comment "a step has a description on how to execute it" ;
  rdfs:label "has step description" .

<http://www.semanticweb.org/joliendeclerck/ontologies/2016/3/OIS-food-ontology#Food>
  a owl:Class ;
  owl:disjointWith <http://www.semanticweb.org/joliendeclerck/ontologies/2016/3/OIS-food-ontology#IngredientQuantity>, <http://www.semanticweb.org/joliendeclerck/ontologies/2016/3/OIS-food-ontology#NutritiveValue>, <http://www.semanticweb.org/joliendeclerck/ontologies/2016/3/OIS-food-ontology#NutritiveValueQuantity>, <http://www.semanticweb.org/joliendeclerck/ontologies/2016/3/OIS-food-ontology#Recipe>, <http://www.semanticweb.org/joliendeclerck/ontologies/2016/3/OIS-food-ontology#RecipeStep> ;
  rdfs:comment "Any substance that can be eaten or drunk. When consumed, it provides a nutrition. Food can be an ingredient or the result of a recipe." ;
  rdfs:label "food" .

<http://www.semanticweb.org/joliendeclerck/ontologies/2016/3/OIS-food-ontology#Ingredient>
  a owl:Class ;
  owl:disjointWith <http://www.semanticweb.org/joliendeclerck/ontologies/2016/3/OIS-food-ontology#IngredientQuantity>, <http://www.semanticweb.org/joliendeclerck/ontologies/2016/3/OIS-food-ontology#NutritiveValueQuantity>, <http://www.semanticweb.org/joliendeclerck/ontologies/2016/3/OIS-food-ontology#Recipe>, <http://www.semanticweb.org/joliendeclerck/ontologies/2016/3/OIS-food-ontology#RecipeStep> ;
  rdfs:comment "An ingredient is a substance containing nutrients; an ingredient can be a food." ;
  rdfs:label "ingredient" .

<http://www.semanticweb.org/joliendeclerck/ontologies/2016/3/OIS-food-ontology#IngredientQuantity>
  a owl:Class ;
  owl:disjointWith <http://www.semanticweb.org/joliendeclerck/ontologies/2016/3/OIS-food-ontology#NutritiveValue>, <http://www.semanticweb.org/joliendeclerck/ontologies/2016/3/OIS-food-ontology#Recipe>, <http://www.semanticweb.org/joliendeclerck/ontologies/2016/3/OIS-food-ontology#RecipeStep> ;
  rdfs:comment """The link between a recipe and an ingredient. 
It depicts the amount of some ingredient necessary to complete a recipe.""" ;
  rdfs:label "ingredient quantity" .

<http://www.semanticweb.org/joliendeclerck/ontologies/2016/3/OIS-food-ontology#NutritiveValue>
  a owl:Class ;
  owl:disjointWith <http://www.semanticweb.org/joliendeclerck/ontologies/2016/3/OIS-food-ontology#NutritiveValueQuantity>, <http://www.semanticweb.org/joliendeclerck/ontologies/2016/3/OIS-food-ontology#Recipe>, <http://www.semanticweb.org/joliendeclerck/ontologies/2016/3/OIS-food-ontology#RecipeStep> ;
  rdfs:comment """A substance that provides nourishment essential for the maintenance of life and for growth. 
For example fat, sugar, carbohydrate, protein, sodium.""" ;
  rdfs:label "nutritive value" .

<http://www.semanticweb.org/joliendeclerck/ontologies/2016/3/OIS-food-ontology#NutritiveValueQuantity>
  a owl:Class ;
  owl:disjointWith <http://www.semanticweb.org/joliendeclerck/ontologies/2016/3/OIS-food-ontology#Recipe>, <http://www.semanticweb.org/joliendeclerck/ontologies/2016/3/OIS-food-ontology#RecipeStep> ;
  rdfs:comment "The quantity and unit of a nutritive value for 100 grams of a certain ingredient." ;
  rdfs:label "nutritive value quantity" .

<http://www.semanticweb.org/joliendeclerck/ontologies/2016/3/OIS-food-ontology#Recipe>
  a owl:Class ;
  owl:disjointWith <http://www.semanticweb.org/joliendeclerck/ontologies/2016/3/OIS-food-ontology#RecipeStep> ;
  rdfs:comment "A collection of ingredients and/or the steps necessary to combine the ingredients into some food." ;
  rdfs:label "recipe" .

<http://www.semanticweb.org/joliendeclerck/ontologies/2016/3/OIS-food-ontology#RecipeStep>
  a owl:Class ;
  rdfs:comment """A step in the preparation process of a recipe. A step has a ordering number starting from 1. 
A step has a number for ordering and a string as a human readable description.""" ;
  rdfs:label "recipe step" .

<http://www.semanticweb.org/joliendeclerck/ontologies/2016/3/OIS-food-ontology#calorie> a owl:NamedIndividual .
<http://www.semanticweb.org/joliendeclerck/ontologies/2016/3/OIS-food-ontology#salt> a owl:NamedIndividual .
<http://www.semanticweb.org/joliendeclerck/ontologies/2016/3/OIS-food-ontology#sugar> a owl:NamedIndividual .
owl:topDataProperty rdfs:comment "" .
